gicSGITargetMaskBits -> gicNumTargets
Signed-off-by: Gerwin Klein <gerwin.klein@proofcraft.systems>

spec/haskell/src/SEL4/Machine/Hardware/AARCH64.hs
@@ -479,8 +479,8 @@ numSGIs :: Int
 numSGIs = error "defined in machine/AARCH64/Platform.thy"
 
 -- SGI targets
-gicSGITargetMaskBits :: Int
-gicSGITargetMaskBits = error "defined in machine/AARCH64/Platform.thy"
+gicNumTargets :: Int
+gicNumTargets = error "defined in machine/AARCH64/Platform.thy"
 
 -- the C bitfield definition reserves 16 bit each in the cap; only 8 bits are used for GICv2
 type SGIIRQ = Word16
