spec/haskell/src/SEL4/Object/Interrupt/AARCH64.hs
@@ -50,7 +50,7 @@ decodeIRQControlInvocation label args srcSlot extraCaps =
         (ArchInvocationLabel ArchLabels.ARMIRQIssueSGISignal,
          irqW:targetsW:index:depth:_, cnode:_) -> do
             rangeCheck irqW 0 (Arch.numSGIs - 1)
-            rangeCheck targetsW 0 (mask Arch.gicSGITargetMaskBits :: Word)
+            rangeCheck targetsW 0 (mask Arch.gicNumTargets :: Word)
             sgiSlot <- lookupTargetSlot cnode (CPtr index) (fromIntegral depth)
             ensureEmptySlot sgiSlot
             return $ ArchInv.IssueSGISignal (fromIntegral irqW) (fromIntegral targetsW)
